proofs/fstar/extraction/Libcrux.Kem.Kyber.Conversions.fst
@@ -3,22 +3,11 @@ module Libcrux.Kem.Kyber.Conversions
 open Core
 open FStar.Mul
 
-class t_UpdatingArray (v_Self: Type) = { f_push:v_Self -> t_Slice u8 -> v_Self }
-
+inline_for_extraction
+class t_UpdatingArray (v_Self: Type) = { f_push:v_Self -> t_Slice u8 -> FStar.HyperStack.ST.St v_Self }
+ 
+inline_for_extraction
 let into_padded_array (v_LEN: usize) (slice: t_Slice u8) : FStar.HyperStack.ST.St (t_Array u8 v_LEN) =
-  let _:Prims.unit =
-    if true
-    then
-      let _:Prims.unit =
-        if ~.((Core.Slice.impl__len slice <: usize) <=. v_LEN <: bool)
-        then
-          Rust_primitives.Hax.never_to_any (Core.Panicking.panic "assertion failed: slice.len() <= LEN"
-
-              <:
-              Rust_primitives.Hax.t_Never)
-      in
-      ()
-  in
   let out:t_Array u8 v_LEN = Rust_primitives.Hax.repeat 0uy v_LEN in
   let _:Prims.unit =
     Core.Slice.impl__copy_from_slice (Core.Ops.Index.f_index_mut out
@@ -34,19 +23,23 @@ let into_padded_array (v_LEN: usize) (slice: t_Slice u8) : FStar.HyperStack.ST.S
   in
   out
 
+inline_for_extraction
 type t_UpdatableArray (v_LEN: usize) = {
   f_value:t_Array u8 v_LEN;
   f_pointer:usize
 }
 
+inline_for_extraction
 let impl__array (v_LEN: usize) (self: t_UpdatableArray v_LEN)
     : FStar.HyperStack.ST.St (t_Array u8 v_LEN) = self.f_value
 
+inline_for_extraction
 let impl__new (v_LEN: usize) (value: t_Array u8 v_LEN)
     : FStar.HyperStack.ST.St (t_UpdatableArray v_LEN) =
   { f_value = value; f_pointer = sz 0 } <: t_UpdatableArray v_LEN
 
 [@@ FStar.Tactics.Typeclasses.tcinstance]
+inline_for_extraction
 let impl_1 (v_LEN: usize) : t_UpdatingArray (t_UpdatableArray v_LEN) =
   {
     f_push
